code/aes/Hacl.Impl.Poly1305.Fields.fst
@@ -6,12 +6,15 @@ open FStar.HyperStack.All
 open Lib.IntTypes
 open LowStar.Buffer
 open Lib.Utils
+open Lib.Vec128
 module F32 = Hacl.Impl.Poly1305.Field32
 module F64 = Hacl.Impl.Poly1305.Field64
+module F128 = Hacl.Impl.Poly1305.Field128
 
 type field_spec = 
   | M32 
   | M64 
+  | M128 
 
 
 unfold
@@ -19,30 +22,35 @@ let limb (s:field_spec) =
   match s with
   | M32 -> uint32
   | M64 -> uint64
+  | M128 -> vec128
 
 unfold
 let limb_zero (s:field_spec) : limb s=
   match s with
   | M32 -> u32 0 
   | M64 -> u64 0
+  | M128 -> vec128_zero
 
 unfold
 let wide (s:field_spec) =
   match s with
   | M32 -> uint64
   | M64 -> uint128
+  | M128 -> vec128
 
 unfold
 let nlimb (s:field_spec) : size_nat =
   match s with
   | M32 -> 5
   | M64 -> 3
+  | M128 -> 5
 
 unfold
 let blocklen (s:field_spec) : size_nat =
   match s with
-  | M32 -> 1
-  | M64 -> 1
+  | M32 -> 16
+  | M64 -> 16
+  | M128 -> 32
 
 
 type felem (s:field_spec) = lbuffer (limb s) (nlimb s)
@@ -54,6 +62,7 @@ let as_nat #s h (e:felem s) =
   match s with
   | M32 -> F32.as_nat h e
   | M64 -> F64.as_nat h e
+  | M128 -> admit()
   
 inline_for_extraction
 val create_felem: s:field_spec -> StackInline (felem s)
@@ -64,6 +73,7 @@ let create_felem s =
   match s with
   | M32 -> (F32.create_felem ()) <: felem s
   | M64 -> (F64.create_felem ()) <: felem s
+  | M128 -> (F128.create_felem ()) <: felem s
 
 
 inline_for_extraction
@@ -74,6 +84,7 @@ let load_felem_le (#s:field_spec) (f:felem s) (b:lbytes 16) =
   match s with
   | M32 -> F32.load_felem_le f b
   | M64 -> F64.load_felem_le f b
+  | M128 -> F128.load_felem_le f b
 
 inline_for_extraction
 val store_felem_le: #s:field_spec -> b:lbytes 16 -> f:felem s -> Stack unit
@@ -83,6 +94,7 @@ let store_felem_le #s b f =
   match s with
   | M32 -> F32.store_felem_le b f 
   | M64 -> F64.store_felem_le b f 
+  | M128 -> F128.store_felem_le b f 
 
 inline_for_extraction
 val set_bit: #s:field_spec -> f:felem s -> i:size_t{size_v i < 130} -> Stack unit
@@ -92,6 +104,7 @@ let set_bit (#s:field_spec) (f:felem s) (i:size_t{size_v i < 130}) =
   match s with
   | M32 -> F32.set_bit f i
   | M64 -> F64.set_bit f i
+  | M128 -> F128.set_bit f i
 
 inline_for_extraction
 val set_bit128: #s:field_spec -> f:felem s -> Stack unit
@@ -101,6 +114,7 @@ let set_bit128 (#s:field_spec) (f:felem s) =
   match s with
   | M32 -> F32.set_bit128 f
   | M64 -> F64.set_bit128 f
+  | M128 -> F128.set_bit128 f
 
 
 inline_for_extraction
@@ -111,6 +125,17 @@ let set_zero (#s:field_spec) (f:felem s) =
   match s with
   | M32 -> F32.set_zero f
   | M64 -> F64.set_zero f
+  | M128 -> F128.set_zero f
+
+inline_for_extraction
+val copy_felem: #s:field_spec -> f:felem s -> f':felem s -> Stack unit
+                   (requires (fun h -> live h f /\ live h f'))
+		   (ensures (fun h0 _ h1 -> modifies (loc_buffer f) h0 h1))
+let copy_felem (#s:field_spec) (f:felem s) (f':felem s) = 
+  match s with
+  | M32 -> F32.copy_felem f f'
+  | M64 -> F64.copy_felem f f'
+  | M128 -> F128.copy_felem f f'
 
 
 inline_for_extraction
@@ -121,7 +146,8 @@ let reduce_felem #s f =
   match s with
   | M32 -> F32.reduce_felem f
   | M64 -> F64.reduce_felem f
-
+  | M128 -> F128.reduce_felem f
+  
 inline_for_extraction
 val precompute_shift_reduce: #s:field_spec -> f1:felem s -> f2:felem s-> Stack unit
                    (requires (fun h -> live h f1 /\ live h f2))
@@ -130,23 +156,39 @@ let precompute_shift_reduce #s f1 f2 =
   match s with
   | M32 -> F32.precompute_shift_reduce f1 f2
   | M64 -> F64.precompute_shift_reduce f1 f2
+  | M128 -> F128.precompute_shift_reduce f1 f2
 
 
 inline_for_extraction
-val fadd_mul_felem: #s:field_spec -> acc:felem s -> f1:felem s -> f2:felem s -> precomp:felem s -> Stack unit
-                   (requires (fun h -> live h acc /\ live h f1 /\ live h f2 /\ live h precomp))
-		   (ensures (fun h0 _ h1 -> modifies (loc_buffer acc) h0 h1))
-let fadd_mul_felem #s acc f1 f2 precomp =
+val fmul: #s:field_spec -> out:felem s -> f1:felem s -> f2:felem s -> precomp:felem s -> Stack unit
+                   (requires (fun h -> live h out /\ live h f1 /\ live h f2 /\ live h precomp))
+		   (ensures (fun h0 _ h1 -> modifies (loc_buffer out) h0 h1))
+let fmul #s out f1 f2 precomp =
   match s with
-  | M32 -> F32.fadd_mul_felem acc f1 f2 precomp
-  | M64 -> F64.fadd_mul_felem acc f1 f2 precomp
+  | M32 -> F32.fmul out f1 f2 precomp
+  | M64 -> F64.fmul out f1 f2 precomp
+  | M128 -> F128.fmul out f1 f2 precomp
+
 
 inline_for_extraction
-val add_felem: #s:field_spec -> f1:felem s -> f2:felem s -> Stack unit
-                   (requires (fun h -> live h f1 /\ live h f2))
-		   (ensures (fun h0 _ h1 -> modifies (loc_buffer f1) h0 h1))
-let add_felem #s f1 f2=
+val fadd_mul: #s:field_spec -> out:felem s -> f1:felem s -> f2:felem s -> precomp:felem s -> Stack unit
+                   (requires (fun h -> live h out /\ live h f1 /\ live h f2 /\ live h precomp))
+		   (ensures (fun h0 _ h1 -> modifies (loc_buffer out) h0 h1))
+let fadd_mul #s out f1 f2 precomp =
   match s with
-  | M32 -> F32.add_felem f1 f2 
-  | M64 -> F64.add_felem f1 f2 
+  | M32 -> F32.fadd_mul out f1 f2 precomp
+  | M64 -> F64.fadd_mul out f1 f2 precomp
+  | M128 -> F128.fadd_mul out f1 f2 precomp
+
+
+
+inline_for_extraction
+val fadd: #s:field_spec -> out:felem s -> f1:felem s -> f2:felem s -> Stack unit
+                   (requires (fun h -> live h out /\ live h f1 /\ live h f2))
+		   (ensures (fun h0 _ h1 -> modifies (loc_buffer out) h0 h1))
+let fadd #s out f1 f2=
+  match s with
+  | M32 -> F32.fadd out f1 f2 
+  | M64 -> F64.fadd out f1 f2 
+  | M128 -> F128.fadd out f1 f2 
 
